Addition_Hoare.thy
@@ -1,0 +1,982 @@
+(*
+ * Copyright 2019, NTU
+ *
+ * This software may be distributed and modified according to the terms of
+ * the BSD 2-Clause license. Note that NO WARRANTY is provided.
+ * See "LICENSE_BSD2.txt" for details.
+ *
+ *  Author: Albert Rizaldi, NTU Singapore
+ *)
+
+theory Addition_Hoare
+  imports VHDL_Hoare_Complete Bits_Int_Aux
+begin
+
+datatype sig = A | B | C
+
+definition add :: "sig conc_stmt" where
+  "add \<equiv> process {A, B} : Bassign_trans C (Badd (Bsig A) (Bsig B)) 1"
+
+lemma potential_tyenv:
+  assumes "seq_wt \<Gamma> (Bassign_trans C (Badd (Bsig A) (Bsig B)) 1)"
+  shows "\<exists>len1 len2. \<Gamma> A = Lty Uns len1 \<and> \<Gamma> B = Lty Uns len2 \<and> \<Gamma> C = Lty Uns (max len1 len2)
+                   \<or> \<Gamma> A = Lty Sig len1 \<and> \<Gamma> B = Lty Sig len2 \<and> \<Gamma> C = Lty Sig (max len1 len2)"
+proof (rule seq_wt_cases(4)[OF assms])
+  assume "bexp_wt \<Gamma> (Badd (Bsig A) (Bsig B)) (\<Gamma> C)"
+  obtain len1 len2 where " \<Gamma> A = Lty Uns len1 \<and> \<Gamma> B = Lty Uns len2 \<and> \<Gamma> C = Lty Uns (max len1 len2)
+                              \<or> \<Gamma> A = Lty Sig len1 \<and> \<Gamma> B = Lty Sig len2 \<and> \<Gamma> C = Lty Sig (max len1 len2)"
+    by (rule bexp_wt_cases(11)[OF \<open>bexp_wt \<Gamma> (Badd (Bsig A) (Bsig B)) (\<Gamma> C)\<close>])
+       (metis bexp_wt_cases(9))+
+  thus ?thesis
+    by auto
+qed
+
+locale unsigned_addition =
+  fixes \<Gamma> :: "sig tyenv"
+  fixes len len1 len2 :: nat
+  assumes len_def: "len = max len1 len2"
+  assumes atype: "\<Gamma> A = Lty Uns len1" and btype: "\<Gamma> B = Lty Uns len2" and ctype: "\<Gamma> C = Lty Uns len"
+begin
+
+lemma well_typed:
+  "seq_wt \<Gamma> (Bassign_trans C (Badd (Bsig A) (Bsig B)) 1)"
+  apply (rule seq_wt.intros(4))
+  unfolding ctype len_def apply (rule bexp_wt.intros(15))
+  unfolding atype[THEN sym] btype[THEN sym]
+  by (rule bexp_wt.intros(3))+
+
+abbreviation "lof_wline tw sig n \<equiv> lval_of (wline_of tw sig n)"
+
+term "bin_to_bl len (bl_to_bin bs1 + bl_to_bin bs2)"
+
+text \<open>Here we factor out common expression in both inv1 and inv2. It is parametrised by the index
+we are interested with for C (first argument) and A (the second argument). Note that the index
+we are interested with for A should be the same as the index for B.\<close>
+
+definition property :: "nat \<Rightarrow> nat \<Rightarrow> sig assn2" where
+  "property idxc idx =
+      (\<lambda>tw. lof_wline tw C idxc =
+                  bin_to_bl len (bl_to_bin (lof_wline tw A idx) + bl_to_bin (lof_wline tw B idx)))"
+
+definition inv :: "sig assn2" where
+  "inv tw \<equiv> (\<forall>i < fst tw. property (i + 1) i tw)"
+
+definition inv2 :: "sig assn2" where
+  "inv2 tw \<equiv> (disjnt {A, B} (event_of tw) \<longrightarrow> (\<forall>i \<ge> fst tw. property (i + 1) (fst tw) tw))"
+
+abbreviation "next_world tw \<equiv> (next_time_world tw, snd tw)"
+
+lemma inv_next_time:
+  assumes "inv tw"
+  assumes "beval_world_raw2 tw (Badd (Bsig A) (Bsig B)) v" and "type_of v = Lty Uns len"
+  defines "tw' \<equiv> tw[C, 1 :=\<^sub>2 v]"
+  shows   "inv (next_time_world tw', snd tw')"
+  unfolding inv_def
+proof (rule, rule)
+  fix i
+  assume "i < fst (next_world tw')"
+  hence "i < next_time_world tw'"
+    by auto
+  have "fst tw' < next_time_world tw'"
+    using next_time_world_at_least  using nat_less_le by blast
+  moreover have "fst tw = fst tw'"
+    unfolding tw'_def worldline_upd2_def worldline_upd_def by auto
+  ultimately have "fst tw < next_time_world tw'"
+    by auto
+  hence "i < fst tw \<or> fst tw \<le> i \<and> i < next_time_world tw' - 1 \<or> i = next_time_world tw' - 1"
+    using \<open>i < next_time_world tw'\<close> by linarith
+  moreover
+  { assume "i < fst tw"
+    have "lof_wline tw' C (i + 1) = lof_wline tw C (i + 1)"
+      by (metis \<open>i < get_time tw\<close> add_mono1 tw'_def worldline_upd2_before_dly)
+    also have "... = bin_to_bl len (bl_to_bin (lof_wline tw A i) + bl_to_bin (lof_wline tw B i))"
+      using assms(1) \<open>i < fst tw\<close> unfolding inv_def property_def by auto
+    also have "... = bin_to_bl len (bl_to_bin (lof_wline tw' A i) + bl_to_bin (lof_wline tw' B i))"
+      by (metis \<open>i < get_time tw\<close> add.commute trans_less_add2 tw'_def worldline_upd2_before_dly)
+    finally have "property (i + 1) i (next_time_world tw', snd tw')"
+      unfolding property_def by auto }
+  moreover
+  { assume "fst tw \<le> i \<and> i < next_time_world tw' - 1"
+    hence "fst tw \<le> i" and "i < next_time_world tw' - 1"
+      by auto
+    hence "lof_wline tw' C (i + 1) = lof_wline tw' C (fst tw + 1)"
+      using unchanged_until_next_time_world
+      by (metis (mono_tags, lifting) Suc_eq_plus1 \<open>get_time tw = get_time tw'\<close> le_Suc_eq le_add1
+          le_less_trans less_diff_conv)
+    moreover have "lof_wline tw' A i = lof_wline tw' A (fst tw)" and "lof_wline tw' B i = lof_wline tw' B (fst tw)"
+      using unchanged_until_next_time_world
+      by (metis \<open>get_time tw = get_time tw'\<close> \<open>get_time tw \<le> i\<close> \<open>i < next_time_world tw'\<close>
+      less_add_one tw'_def worldline_upd2_before_dly)+
+    moreover have "property (fst tw + 1) (fst tw) tw'"
+    proof -
+      have assm2: "beval_world_raw (snd tw) (fst tw) (Badd (Bsig A) (Bsig B)) v"
+        using assms(2) unfolding beval_world_raw2_def by auto
+      have "wline_of tw' C (fst tw + 1) = v"
+        unfolding tw'_def worldline_upd2_def worldline_upd_def by auto
+      also have "... =  Lv Uns (bin_to_bl_aux len (bl_to_bin (lof_wline tw A (fst tw)) + bl_to_bin (lof_wline tw B (fst tw))) [])"
+        apply (rule beval_world_raw_cases[OF assm2])
+        apply ( erule beval_cases)+
+        unfolding state_of_world_def using atype btype
+        apply (metis assms(3) bin_to_bl_def comp_def size_bin_to_bl ty.inject type_of.simps(2) val.sel(3))
+        using assms(3) by auto
+      also have "... =  Lv Uns (bin_to_bl_aux len (bl_to_bin (lof_wline tw' A (fst tw)) + bl_to_bin (lof_wline tw' B (fst tw))) [])"
+        by (metis Suc_eq_plus1 \<open>lval_of (wline_of tw' A i) = lval_of (wline_of tw' A (get_time tw))\<close>
+        \<open>lval_of (wline_of tw' B i) = lval_of (wline_of tw' B (get_time tw))\<close> lessI tw'_def
+        worldline_upd2_before_dly)
+      finally show ?thesis
+        unfolding property_def bin_to_bl_def by auto
+    qed
+    ultimately have "property (i + 1) i (next_world tw')"
+      unfolding property_def by auto }
+  moreover
+  { assume "i = next_time_world tw' - 1"
+    hence "lof_wline tw' C (i + 1) = lof_wline tw' C (next_time_world tw')"
+      using \<open>i < next_time_world tw'\<close> by force
+    also have "... = lof_wline tw' C (fst tw + 1)"
+      using \<open>fst tw < next_time_world tw'\<close> unfolding tw'_def worldline_upd2_def
+      worldline_upd_def by auto
+    finally have "lof_wline tw' C (i + 1) = lof_wline tw' C (fst tw + 1)"
+      by auto
+    moreover have "property (fst tw + 1) (fst tw) tw'"
+    proof -
+      have assm2: "beval_world_raw (snd tw) (fst tw) (Badd (Bsig A) (Bsig B)) v"
+        using assms(2) unfolding beval_world_raw2_def by auto
+      have "wline_of tw' C (fst tw + 1) = v"
+        unfolding tw'_def worldline_upd2_def worldline_upd_def by auto
+      also have "... =  Lv Uns (bin_to_bl_aux len (bl_to_bin (lof_wline tw A (fst tw)) + bl_to_bin (lof_wline tw B (fst tw))) [])"
+        apply (rule beval_world_raw_cases[OF assm2])
+        apply ( erule beval_cases)+
+        unfolding state_of_world_def using atype btype
+        apply (metis assms(3) bin_to_bl_def comp_def size_bin_to_bl ty.inject type_of.simps(2) val.sel(3))
+        using assms(3) by auto
+      also have "... =  Lv Uns (bin_to_bl_aux len (bl_to_bin (lof_wline tw' A (fst tw)) + bl_to_bin (lof_wline tw' B (fst tw))) [])"
+        by (metis less_add_one tw'_def worldline_upd2_before_dly)
+      finally show ?thesis
+        unfolding property_def bin_to_bl_def by auto
+    qed
+    moreover have "lof_wline tw' A i = lof_wline tw' A (fst tw)" and "lof_wline tw' B i = lof_wline tw' B (fst tw)"
+      using unchanged_until_next_time_world
+      by (metis \<open>get_time tw < next_time_world tw'\<close> \<open>get_time tw = get_time tw'\<close> \<open>i <
+      next_time_world tw'\<close> \<open>i = next_time_world tw' - 1\<close> add_le_imp_le_diff discrete)+
+    ultimately have "property (i + 1) i (next_world tw')"
+      unfolding property_def by auto }
+  ultimately show "property (i + 1) i (next_world tw')"
+    by auto
+qed
+
+lemma type_correctness_length:
+  assumes "wityping \<Gamma> (snd tw)"
+  assumes "beval_world_raw2 tw (Badd (Bsig A) (Bsig B)) v"
+  shows   "type_of v = Lty Uns len"
+proof -
+  have "beval_world_raw (snd tw) (fst tw) (Badd (Bsig A) (Bsig B)) v"
+    using assms(2) unfolding beval_world_raw2_def by auto
+  have "type_of (state_of_world (snd tw) (fst tw) A) = Lty Uns len1" and
+       "type_of (state_of_world (snd tw) (fst tw) B) = Lty Uns len2"
+    using assms(1) unfolding wityping_def
+    by (simp add: atype btype state_of_world_def wtyping_def)+
+  show ?thesis
+    apply (rule beval_world_raw_cases[OF \<open>beval_world_raw (snd tw) (fst tw) (Badd (Bsig A) (Bsig B)) v\<close>])
+    apply (erule beval_cases)
+    apply (metis (no_types, lifting) \<open>type_of (state_of_world (snd tw) (get_time tw) A) = Lty Uns len1\<close> \<open>type_of (state_of_world (snd tw) (get_time tw) B) = Lty Uns len2\<close> add.right_neutral beval_cases(1) len_def list.size(3) size_bin_to_bl_aux ty.inject type_of.simps(2))
+    apply (metis (no_types, lifting) \<open>type_of (state_of_world (snd tw) (get_time tw) A) = Lty Uns len1\<close> beval_cases(1) signedness.distinct(5) ty.inject type_of.simps(2))
+    done
+qed
+
+lemma add_seq_hoare_next_time:
+  "\<turnstile> [\<lambda>tw. inv tw \<and> wityping \<Gamma> (snd tw)]
+        Bassign_trans C (Badd (Bsig A) (Bsig B)) 1
+     [\<lambda>tw. inv (next_world tw)]"
+  apply (rule Conseq2[where Q="\<lambda>tw. inv (next_world tw) \<and> wityping \<Gamma> (snd tw)", rotated 1], rule Assign2, simp)
+  using inv_next_time type_correctness_length
+  by (metis ctype snd_conv worldline_upd2_def worldline_upd_preserve_wityping)
+
+lemma add_seq_hoare_next_time0:
+  "\<turnstile> [\<lambda>tw. fst tw = 0 \<and> wityping \<Gamma> (snd tw)]
+        Bassign_trans C (Badd (Bsig A) (Bsig B)) 1
+     [\<lambda>tw. inv (next_world tw)]"
+  apply (rule Conseq2[where Q="\<lambda>tw. inv (next_world tw) \<and> wityping \<Gamma> (snd tw)", rotated 1], rule Assign2, simp)
+  using inv_next_time type_correctness_length unfolding inv_def
+  by (metis ctype gr_implies_not0 snd_conv worldline_upd2_def worldline_upd_preserve_wityping)
+
+lemma add_conc_hoare:
+  "\<And>tw. inv tw \<and> inv2 tw \<and> disjnt {A, B} (event_of tw) \<Longrightarrow> inv (next_world tw)"
+proof -
+  fix tw
+  assume "inv tw \<and> inv2 tw \<and> disjnt {A, B} (event_of tw)"
+  hence "inv tw" and "inv2 tw" and "disjnt {A, B} (event_of tw)"
+    by auto
+  { fix i
+    assume "i < next_time_world tw"
+    have "fst tw < next_time_world tw"
+      by (simp add: next_time_world_at_least)
+    have "i < fst tw \<or> fst tw \<le> i"
+      by auto
+    moreover
+    { assume "i < fst tw"
+      hence "property (i + 1) i tw"
+        using \<open>inv tw\<close> unfolding inv_def by auto
+      hence "property (i + 1) i (next_world tw)"
+        unfolding property_def by simp }
+    moreover
+    { assume "fst tw \<le> i"
+      moreover have "\<forall>i \<ge> fst tw. property (i + 1) (fst tw) tw"
+        using \<open>inv2 tw\<close> \<open>disjnt {A, B} (event_of tw)\<close> unfolding inv2_def
+        by auto
+      ultimately have "property (i + 1) (fst tw) tw"
+        by auto
+      hence "property (i + 1) i tw"
+        unfolding property_def
+        by (metis \<open>get_time tw \<le> i\<close> \<open>i < next_time_world tw\<close> unchanged_until_next_time_world)
+      hence "property (i + 1) i (next_world tw)"
+        unfolding property_def by auto }
+    ultimately have "property (i + 1) i (next_world tw)"
+      by auto }
+  thus "inv (next_world tw)"
+    unfolding inv_def by auto
+qed
+
+lemma add_conc_hoare2:
+  "\<And>tw. inv tw \<and> inv2 tw \<and> disjnt {A, B} (event_of tw) \<Longrightarrow> inv2 (next_world tw)"
+proof -
+  fix tw
+  assume "inv tw \<and> inv2 tw \<and> disjnt {A, B} (event_of tw)"
+  hence "inv tw" and "inv2 tw" and "disjnt {A, B} (event_of tw)"
+    by auto
+  let ?t' = "next_time_world tw"
+  { assume "disjnt {A, B} (event_of (next_world tw))"
+    hence *: "lof_wline tw A ?t' = lof_wline tw A (?t' - 1)" and **: "lof_wline tw B ?t' = lof_wline tw B (?t' - 1)"
+      unfolding event_of_alt_def
+      by (smt comp_apply diff_0_eq_0 disjnt_insert1 fst_conv mem_Collect_eq snd_conv)+
+    have "fst tw < ?t'"
+      by (simp add: next_time_world_at_least)
+    { fix i
+      assume "?t' \<le> i"
+      have "property (i + 1) (fst tw) tw"
+        using \<open>inv2 tw\<close> \<open>disjnt {A, B} (event_of tw)\<close> unfolding inv2_def
+        using \<open>get_time tw < next_time_world tw\<close> \<open>next_time_world tw \<le> i\<close> by auto
+      moreover have "lof_wline tw A (fst tw) = lof_wline tw A (?t' - 1)" and
+                    "lof_wline tw B (fst tw) = lof_wline tw B (?t' - 1)"
+        by (metis \<open>get_time tw < next_time_world tw\<close> add_le_imp_le_diff diff_less discrete gr_implies_not0 not_less_iff_gr_or_eq unchanged_until_next_time_world zero_less_one)+
+      ultimately have "property (i + 1) ?t' (next_world tw)"
+        unfolding property_def using * **  by auto }
+    hence "\<forall>i\<ge>?t'. property (i + 1) ?t' (next_world tw)"
+      by auto }
+  thus "inv2 (next_world tw)"
+    unfolding inv2_def by auto
+qed
+
+lemma inv2_next_time:
+  fixes tw
+  assumes "beval_world_raw2 tw (Badd (Bsig A) (Bsig B)) v" and "type_of v = Lty Uns len"
+  defines "tw' \<equiv> tw[C, 1 :=\<^sub>2 v]"
+  shows   "inv2 (next_time_world tw', snd tw')"
+  unfolding inv2_def
+proof (rule, rule, rule)
+  fix i
+  assume "disjnt {A, B} (event_of (next_world tw'))"
+  hence "A \<notin> event_of (next_world tw')" and "B \<notin> event_of (next_world tw')"
+    by auto
+  assume "fst (next_world tw') \<le> i"
+  hence "next_time_world tw' \<le> i"
+    by auto
+  let ?t' = "next_time_world tw'"
+  have "fst tw' < ?t'"
+    using next_time_world_at_least by blast
+  moreover have "fst tw = fst tw'"
+    unfolding tw'_def unfolding worldline_upd2_def by auto
+  ultimately have "fst tw < ?t'"
+    by auto
+  have 0: "wline_of (next_world tw') A ?t' = wline_of tw A (fst tw)"
+  proof -
+    have "wline_of tw' A ?t' = wline_of tw' A (?t' - 1)"
+      using \<open>A \<notin> event_of (next_world tw')\<close> unfolding event_of_alt_def
+      using \<open>get_time tw' < next_time_world tw'\<close> by auto
+    also have " ... = wline_of tw' A (fst tw')"
+      using unchanged_until_next_time_world
+      by (metis (no_types, lifting) Suc_diff_1 \<open>get_time tw' < next_time_world tw'\<close> diff_less
+      gr_implies_not_zero le_0_eq less_Suc_eq_le not_less zero_less_one)
+    also have "... = wline_of tw' A (fst tw)"
+      by (simp add: \<open>get_time tw = get_time tw'\<close>)
+    also have "... = wline_of tw A (fst tw)"
+      unfolding tw'_def worldline_upd2_def worldline_upd_def by auto
+    finally show "wline_of (next_world tw') A ?t' = wline_of tw A (fst tw)"
+      by auto
+  qed
+  have 1: "wline_of (next_world tw') B ?t' = wline_of tw B (fst tw)"
+  proof -
+    have "wline_of tw' B ?t' = wline_of tw' B (?t' - 1)"
+      using \<open>B \<notin> event_of (next_world tw')\<close> unfolding event_of_alt_def
+      using \<open>get_time tw' < next_time_world tw'\<close> by auto
+    also have " ... = wline_of tw' B (fst tw')"
+      using unchanged_until_next_time_world
+      by (metis (no_types, lifting) Suc_diff_1 \<open>get_time tw' < next_time_world tw'\<close> diff_less
+      gr_implies_not_zero le_0_eq less_Suc_eq_le not_less zero_less_one)
+    also have "... = wline_of tw' B (fst tw)"
+      by (simp add: \<open>get_time tw = get_time tw'\<close>)
+    also have "... = wline_of tw B (fst tw)"
+      unfolding tw'_def worldline_upd2_def worldline_upd_def by auto
+    finally show "wline_of (next_world tw') B ?t' = wline_of tw B (fst tw)"
+      by auto
+  qed
+  have assm2: "beval_world_raw (snd tw) (fst tw) (Badd (Bsig A) (Bsig B)) v"
+    using assms(1) unfolding beval_world_raw2_def by auto
+  have "wline_of (next_world tw') C (i + 1) = v"
+  proof -
+    have "wline_of tw' C (i + 1) = v"
+      using `fst tw < ?t'` \<open>?t' \<le> i\<close>
+      unfolding tw'_def worldline_upd2_def worldline_upd_def by auto
+    thus ?thesis
+      by auto
+  qed
+  also have "lval_of ... = bin_to_bl len (bl_to_bin (lof_wline tw A (fst tw)) + bl_to_bin (lof_wline tw B (fst tw)))"
+    apply (rule beval_world_raw_cases[OF assm2])
+    apply (erule beval_cases)+
+    apply (metis assms(2) beval_raw.intros(1) beval_world_raw.simps beval_world_raw2_Bsig beval_world_raw2_def beval_world_raw_deterministic bin_to_bl_def size_bin_to_bl ty.inject type_of.simps(2) val.sel(3))
+    using assms(2) by auto
+  finally have "property (i + 1) ?t' (next_world tw')"
+    unfolding property_def using 0 1  by auto
+  thus "property (i + 1) (get_time (next_time_world tw', snd tw')) (next_time_world tw', snd tw')"
+    by auto
+qed
+
+lemma add_seq_hoare_next_time1:
+  shows "\<turnstile> [\<lambda>tw. wityping \<Gamma> (snd tw)] Bassign_trans C (Badd (Bsig A) (Bsig B)) 1 [\<lambda>tw. inv2 (next_time_world tw, snd tw)]"
+  apply (rule Assign2_altI)
+  using inv2_next_time type_correctness_length by blast
+
+lemma add_conc_hoare3:
+  "\<turnstile> \<lbrace>\<lambda>tw. (inv tw \<and> wityping \<Gamma> (snd tw)) \<and> inv2 tw\<rbrace> add \<lbrace>\<lambda>tw. inv (next_time_world tw, snd tw) \<and> inv2 (next_time_world tw, snd tw)\<rbrace>"
+  unfolding add_def
+  apply (rule Single)
+   apply (rule Conj)
+    apply (rule strengthen_precondition)
+  apply (rule strengthen_precondition)
+    apply (rule add_seq_hoare_next_time)
+  apply (rule strengthen_precondition)
+   apply (rule strengthen_precondition)
+   apply (rule strengthen_precondition2)
+   apply (rule add_seq_hoare_next_time1)
+  using add_conc_hoare add_conc_hoare2 by blast
+
+lemma seq_wt_add:
+  "seq_wt \<Gamma> (Bassign_trans C (Badd (Bsig A) (Bsig B)) 1)"
+  using well_typed by blast
+
+lemma add_conc_hoare4:
+  "\<turnstile> \<lbrace>\<lambda>tw. (inv tw \<and> wityping \<Gamma> (snd tw)) \<and> inv2 tw\<rbrace> add \<lbrace>\<lambda>tw. (inv (next_time_world tw, snd tw) \<and> wityping \<Gamma> (snd tw)) \<and> inv2 (next_time_world tw, snd tw)\<rbrace>"
+  apply (rule Conj2)
+   apply (rule Conj2)
+    apply (rule weaken_post_conc_hoare[OF _ add_conc_hoare3], blast)
+   apply (rule strengthen_pre_conc_hoare[rotated])
+    apply (unfold add_def, rule single_conc_stmt_preserve_wityping_hoare)
+    apply (rule seq_wt_add)
+   apply blast
+  apply (fold add_def, rule weaken_post_conc_hoare[OF _ add_conc_hoare3], blast)
+  done
+
+lemma add_conc_sim':
+  "\<turnstile>\<^sub>s \<lbrace>\<lambda>tw. (inv tw \<and> wityping \<Gamma> (snd tw)) \<and> inv2 tw\<rbrace> add \<lbrace>\<lambda>tw. (inv tw \<and> wityping \<Gamma> (snd tw)) \<and> inv2 tw\<rbrace>"
+  apply (rule While)
+  apply (unfold snd_conv, rule add_conc_hoare4)
+  done
+
+lemma add_conc_sim2:
+  "\<turnstile>\<^sub>s \<lbrace>\<lambda>tw. (inv tw \<and> wityping \<Gamma> (snd tw)) \<and> inv2 tw\<rbrace> add \<lbrace>inv\<rbrace>"
+  using add_conc_sim' Conseq_sim by blast
+
+lemma init_sat_add_inv:
+  "init_sim_hoare (\<lambda>tw. fst tw = 0 \<and> wityping \<Gamma> (snd tw)) add (\<lambda>tw. inv tw \<and> wityping \<Gamma> (snd tw))"
+  unfolding add_def
+  apply (rule AssignI)
+  apply (rule SingleI)
+  apply (rule Conj)
+  unfolding snd_conv apply(rule add_seq_hoare_next_time0)
+  apply (rule strengthen_precondition2)
+  by (metis seq_stmt_preserve_wityping_hoare well_typed)
+
+lemma init_sat_add_inv2:
+  "init_sim_hoare (\<lambda>tw. wityping \<Gamma> (snd tw)) add inv2"
+  unfolding add_def
+  apply (rule AssignI)
+  apply (rule SingleI)
+  unfolding snd_conv apply (rule add_seq_hoare_next_time1)
+  done
+
+lemma init_sat_add_inv_comb:
+  shows "init_sim_hoare (\<lambda>tw. fst tw = 0 \<and> wityping \<Gamma> (snd tw)) add  (\<lambda>tw. (inv tw \<and> wityping \<Gamma> (snd tw)) \<and> inv2 tw)"
+  apply (rule ConjI_sim)
+  apply (rule init_sat_add_inv)
+  apply (rule ConseqI_sim[rotated])
+  apply (rule init_sat_add_inv2)
+  by blast+
+
+lemma add_correctness:
+  assumes "sim_fin w (i + 1) add tw'" and "wityping \<Gamma> w"
+  shows   "property (i + 1) i tw'"
+proof -
+  obtain tw where "init_sim (0, w) add tw" and  "tw, i + 1, add \<Rightarrow>\<^sub>S tw'"
+    using premises_sim_fin_obt[OF assms(1)] by auto
+  hence "i + 1 < fst tw'"
+    using world_maxtime_lt_fst_tres  by blast
+  have "conc_stmt_wf add"
+    unfolding conc_stmt_wf_def add_def by auto
+  moreover have "nonneg_delay_conc add"
+    unfolding add_def by auto
+  ultimately have "init_sim_valid (\<lambda>tw. fst tw = 0 \<and> wityping \<Gamma> (snd tw)) add (\<lambda>tw. (inv tw \<and> wityping \<Gamma> (snd tw)) \<and> inv2 tw)"
+    using init_sim_hoare_soundness[OF init_sat_add_inv_comb]
+    by (metis (no_types, lifting) conc_wt_cases(1) init_sat_add_inv_comb
+    init_sim_hoare_soundness add_def strengthen_precondition_init_sim_hoare)
+  hence "inv tw \<and> wityping \<Gamma> (snd tw) \<and> inv2 tw"
+    using \<open>init_sim (0, w) add tw\<close> fst_conv assms(2) unfolding init_sim_valid_def
+    by (metis snd_conv)
+  hence "inv tw" and "inv2 tw" and "wityping \<Gamma> (snd tw)"
+    by auto
+  moreover have "\<Turnstile>\<^sub>s \<lbrace>\<lambda>tw. (inv tw \<and> wityping \<Gamma> (snd tw)) \<and> inv2 tw\<rbrace> add \<lbrace>inv\<rbrace>"
+    using conc_sim_soundness[OF add_conc_sim2] \<open>conc_stmt_wf add\<close> \<open>nonneg_delay_conc add\<close>
+    by auto
+  ultimately have "inv tw'"
+    using \<open>tw, i + 1, add \<Rightarrow>\<^sub>S tw'\<close> unfolding sim_hoare_valid_def by blast
+  with \<open>i + 1 < fst tw'\<close> show ?thesis
+    unfolding inv_def by auto
+qed
+
+corollary add_correctness2:
+  assumes "sim_fin w (i + 1) add tw'" and "wityping \<Gamma> w"
+  defines "bsA \<equiv> lof_wline tw' A i"
+  defines "bsB \<equiv> lof_wline tw' B i"
+  defines "bsC \<equiv> lof_wline tw' C (i + 1)"
+  assumes "bl_to_bin bsA + bl_to_bin bsB < 2 ^ len"
+  shows   "(\<Sum>i = 0..<length bsC. (int \<circ> of_bool) (rev bsC ! i) * 2 ^ i) =
+           (\<Sum>i = 0..<length bsA. (int \<circ> of_bool) (rev bsA ! i) * 2 ^ i) +
+           (\<Sum>i = 0..<length bsB. (int \<circ> of_bool) (rev bsB ! i) * 2 ^ i) "
+           (is "?repC = ?repA + ?repB")
+proof -
+  have "property (i + 1) i tw'"
+    using add_correctness[OF assms(1-2)] by auto
+  hence "lof_wline tw' C (i + 1) =
+                  bin_to_bl len (bl_to_bin (lof_wline tw' A i) + bl_to_bin (lof_wline tw' B i))"
+    unfolding property_def by auto
+  hence "bsC = bin_to_bl len (bl_to_bin bsA + bl_to_bin bsB)" (is "_ = ?rhs")
+    unfolding bsA_def bsB_def bsC_def by auto
+  hence "bl_to_bin bsC = bl_to_bin ?rhs"
+    by auto
+  also have "... = bintrunc len (bl_to_bin bsA + bl_to_bin bsB)"
+    unfolding bin_bl_bin by auto
+  also have "... = (bl_to_bin bsA + bl_to_bin bsB) mod 2 ^ len"
+    unfolding bintrunc_mod2p by auto
+  also have "... = bl_to_bin bsA + bl_to_bin bsB"
+    using assms(6) by (simp add: bl_to_bin_ge0)
+  finally have "bl_to_bin bsC = bl_to_bin bsA + bl_to_bin bsB"
+    by auto
+  thus ?thesis
+    unfolding bl_to_bin_correctness by auto
+qed
+
+end
+
+locale signed_addition =
+  fixes \<Gamma> :: "sig tyenv"
+  fixes len len1 len2 :: nat
+  assumes len_def: "len = max len1 len2"
+  assumes atype: "\<Gamma> A = Lty Sig len1" and btype: "\<Gamma> B = Lty Sig len2" and ctype: "\<Gamma> C = Lty Sig len"
+begin
+
+lemma well_typed:
+  "seq_wt \<Gamma> (Bassign_trans C (Badd (Bsig A) (Bsig B)) 1)"
+  by (rule seq_wt.intros(4))
+     (metis atype bexp_wt.intros(16) bexp_wt.intros(3) btype ctype len_def)
+
+abbreviation "lof_wline tw sig n \<equiv> lval_of (wline_of tw sig n)"
+
+text \<open>Here we factor out common expression in both inv1 and inv2. It is parametrised by the index
+we are interested with for C (first argument) and A (the second argument). Note that the index
+we are interested with for A should be the same as the index for B.\<close>
+
+definition property :: "nat \<Rightarrow> nat \<Rightarrow> sig assn2" where
+  "property idxc idx =
+      (\<lambda>tw. lof_wline tw C idxc =
+                  bin_to_bl len (sbl_to_bin (lof_wline tw A idx) + sbl_to_bin (lof_wline tw B idx)))"
+
+definition inv :: "sig assn2" where
+  "inv tw \<equiv> (\<forall>i < fst tw. property (i + 1) i tw)"
+
+definition inv2 :: "sig assn2" where
+  "inv2 tw \<equiv> (disjnt {A, B} (event_of tw) \<longrightarrow> (\<forall>i \<ge> fst tw. property (i + 1) (fst tw) tw))"
+
+abbreviation "next_world tw \<equiv> (next_time_world tw, snd tw)"
+
+lemma inv_next_time:
+  assumes "inv tw"
+  assumes "beval_world_raw2 tw (Badd (Bsig A) (Bsig B)) v" and "type_of v = Lty Sig len"
+  defines "tw' \<equiv> tw[C, 1 :=\<^sub>2 v]"
+  shows   "inv (next_time_world tw', snd tw')"
+  unfolding inv_def
+proof (rule, rule)
+  fix i
+  assume "i < fst (next_world tw')"
+  hence "i < next_time_world tw'"
+    by auto
+  have "fst tw' < next_time_world tw'"
+    using next_time_world_at_least  using nat_less_le by blast
+  moreover have "fst tw = fst tw'"
+    unfolding tw'_def worldline_upd2_def worldline_upd_def by auto
+  ultimately have "fst tw < next_time_world tw'"
+    by auto
+  hence "i < fst tw \<or> fst tw \<le> i \<and> i < next_time_world tw' - 1 \<or> i = next_time_world tw' - 1"
+    using \<open>i < next_time_world tw'\<close> by linarith
+  moreover
+  { assume "i < fst tw"
+    have "lof_wline tw' C (i + 1) = lof_wline tw C (i + 1)"
+      by (metis \<open>i < get_time tw\<close> add_mono1 tw'_def worldline_upd2_before_dly)
+    also have "... = bin_to_bl len (sbl_to_bin (lof_wline tw A i) + sbl_to_bin (lof_wline tw B i))"
+      using assms(1) \<open>i < fst tw\<close> unfolding inv_def property_def by auto
+    also have "... = bin_to_bl len (sbl_to_bin (lof_wline tw' A i) + sbl_to_bin (lof_wline tw' B i))"
+      by (metis \<open>i < get_time tw\<close> add.commute trans_less_add2 tw'_def worldline_upd2_before_dly)
+    finally have "property (i + 1) i (next_time_world tw', snd tw')"
+      unfolding property_def by auto }
+  moreover
+  { assume "fst tw \<le> i \<and> i < next_time_world tw' - 1"
+    hence "fst tw \<le> i" and "i < next_time_world tw' - 1"
+      by auto
+    hence "lof_wline tw' C (i + 1) = lof_wline tw' C (fst tw + 1)"
+      using unchanged_until_next_time_world
+      by (metis (mono_tags, lifting) Suc_eq_plus1 \<open>get_time tw = get_time tw'\<close> le_Suc_eq le_add1
+          le_less_trans less_diff_conv)
+    moreover have "lof_wline tw' A i = lof_wline tw' A (fst tw)" and "lof_wline tw' B i = lof_wline tw' B (fst tw)"
+      using unchanged_until_next_time_world
+      by (metis \<open>get_time tw = get_time tw'\<close> \<open>get_time tw \<le> i\<close> \<open>i < next_time_world tw'\<close>
+      less_add_one tw'_def worldline_upd2_before_dly)+
+    moreover have "property (fst tw + 1) (fst tw) tw'"
+    proof -
+      have assm2: "beval_world_raw (snd tw) (fst tw) (Badd (Bsig A) (Bsig B)) v"
+        using assms(2) unfolding beval_world_raw2_def by auto
+      have "wline_of tw' C (fst tw + 1) = v"
+        unfolding tw'_def worldline_upd2_def worldline_upd_def by auto
+      also have "... =  Lv Sig (bin_to_bl_aux len (sbl_to_bin (lof_wline tw A (fst tw)) + sbl_to_bin (lof_wline tw B (fst tw))) [])"
+        apply (rule beval_world_raw_cases[OF assm2])
+        apply ( erule beval_cases)
+        defer
+        apply ( erule beval_cases)+
+        unfolding state_of_world_def using atype btype
+        apply (metis assms(3) bin_to_bl_def comp_apply size_bin_to_bl ty.inject type_of.simps(2) val.sel(3))
+        using assms(3) by auto
+      also have "... =  Lv Sig (bin_to_bl_aux len (sbl_to_bin (lof_wline tw' A (fst tw)) + sbl_to_bin (lof_wline tw' B (fst tw))) [])"
+        by (metis Suc_eq_plus1 \<open>lval_of (wline_of tw' A i) = lval_of (wline_of tw' A (get_time tw))\<close>
+        \<open>lval_of (wline_of tw' B i) = lval_of (wline_of tw' B (get_time tw))\<close> lessI tw'_def
+        worldline_upd2_before_dly)
+      finally show ?thesis
+        unfolding property_def bin_to_bl_def by auto
+    qed
+    ultimately have "property (i + 1) i (next_world tw')"
+      unfolding property_def by auto }
+  moreover
+  { assume "i = next_time_world tw' - 1"
+    hence "lof_wline tw' C (i + 1) = lof_wline tw' C (next_time_world tw')"
+      using \<open>i < next_time_world tw'\<close> by force
+    also have "... = lof_wline tw' C (fst tw + 1)"
+      using \<open>fst tw < next_time_world tw'\<close> unfolding tw'_def worldline_upd2_def
+      worldline_upd_def by auto
+    finally have "lof_wline tw' C (i + 1) = lof_wline tw' C (fst tw + 1)"
+      by auto
+    moreover have "property (fst tw + 1) (fst tw) tw'"
+    proof -
+      have assm2: "beval_world_raw (snd tw) (fst tw) (Badd (Bsig A) (Bsig B)) v"
+        using assms(2) unfolding beval_world_raw2_def by auto
+      have "wline_of tw' C (fst tw + 1) = v"
+        unfolding tw'_def worldline_upd2_def worldline_upd_def by auto
+      also have "... =  Lv Sig (bin_to_bl_aux len (sbl_to_bin (lof_wline tw A (fst tw)) + sbl_to_bin (lof_wline tw B (fst tw))) [])"
+        apply (rule beval_world_raw_cases[OF assm2])
+        apply ( erule beval_cases)
+        defer
+        apply ( erule beval_cases)+
+        unfolding state_of_world_def using atype btype
+        apply (metis assms(3) bin_to_bl_def comp_def size_bin_to_bl ty.inject type_of.simps(2) val.sel(3))
+        using assms(3) by auto
+      also have "... =  Lv Sig (bin_to_bl_aux len (sbl_to_bin (lof_wline tw' A (fst tw)) + sbl_to_bin (lof_wline tw' B (fst tw))) [])"
+        by (metis less_add_one tw'_def worldline_upd2_before_dly)
+      finally show ?thesis
+        unfolding property_def bin_to_bl_def by auto
+    qed
+    moreover have "lof_wline tw' A i = lof_wline tw' A (fst tw)" and "lof_wline tw' B i = lof_wline tw' B (fst tw)"
+      using unchanged_until_next_time_world
+      by (metis \<open>get_time tw < next_time_world tw'\<close> \<open>get_time tw = get_time tw'\<close> \<open>i <
+      next_time_world tw'\<close> \<open>i = next_time_world tw' - 1\<close> add_le_imp_le_diff discrete)+
+    ultimately have "property (i + 1) i (next_world tw')"
+      unfolding property_def by auto }
+  ultimately show "property (i + 1) i (next_world tw')"
+    by auto
+qed
+
+lemma type_correctness_length:
+  assumes "wityping \<Gamma> (snd tw)"
+  assumes "beval_world_raw2 tw (Badd (Bsig A) (Bsig B)) v"
+  shows   "type_of v = Lty Sig len"
+proof -
+  have "beval_world_raw (snd tw) (fst tw) (Badd (Bsig A) (Bsig B)) v"
+    using assms(2) unfolding beval_world_raw2_def by auto
+  have "type_of (state_of_world (snd tw) (fst tw) A) = Lty Sig len1" and
+       "type_of (state_of_world (snd tw) (fst tw) B) = Lty Sig len2"
+    using assms(1) unfolding wityping_def
+    by (simp add: atype btype state_of_world_def wtyping_def)+
+  show ?thesis
+    apply (rule beval_world_raw_cases[OF \<open>beval_world_raw (snd tw) (fst tw) (Badd (Bsig A) (Bsig B)) v\<close>])
+    apply (erule beval_cases)
+    apply (metis (no_types, hide_lams) \<open>type_of (state_of_world (snd tw) (get_time tw) A) = Lty Sig len1\<close> beval_cases(1) signedness.distinct(5) ty.inject type_of.simps(2))
+    apply (metis \<open>type_of (state_of_world (snd tw) (get_time tw) A) = Lty Sig len1\<close> \<open>type_of (state_of_world (snd tw) (get_time tw) B) = Lty Sig len2\<close> beval_cases(1) bin_to_bl_def len_def size_bin_to_bl ty.inject type_of.simps(2) val.sel(3))
+    done
+qed
+
+lemma add_seq_hoare_next_time:
+  "\<turnstile> [\<lambda>tw. inv tw \<and> wityping \<Gamma> (snd tw)]
+        Bassign_trans C (Badd (Bsig A) (Bsig B)) 1
+     [\<lambda>tw. inv (next_world tw)]"
+  apply (rule Conseq2[where Q="\<lambda>tw. inv (next_world tw) \<and> wityping \<Gamma> (snd tw)", rotated 1], rule Assign2, simp)
+  using inv_next_time type_correctness_length
+  by (metis ctype snd_conv worldline_upd2_def worldline_upd_preserve_wityping)
+
+lemma add_seq_hoare_next_time0:
+  "\<turnstile> [\<lambda>tw. fst tw = 0 \<and> wityping \<Gamma> (snd tw)]
+        Bassign_trans C (Badd (Bsig A) (Bsig B)) 1
+     [\<lambda>tw. inv (next_world tw)]"
+  apply (rule Conseq2[where Q="\<lambda>tw. inv (next_world tw) \<and> wityping \<Gamma> (snd tw)", rotated 1], rule Assign2, simp)
+  using inv_next_time type_correctness_length unfolding inv_def
+  by (metis ctype gr_implies_not0 snd_conv worldline_upd2_def worldline_upd_preserve_wityping)
+
+lemma add_conc_hoare:
+  "\<And>tw. inv tw \<and> inv2 tw \<and> disjnt {A, B} (event_of tw) \<Longrightarrow> inv (next_world tw)"
+proof -
+  fix tw
+  assume "inv tw \<and> inv2 tw \<and> disjnt {A, B} (event_of tw)"
+  hence "inv tw" and "inv2 tw" and "disjnt {A, B} (event_of tw)"
+    by auto
+  { fix i
+    assume "i < next_time_world tw"
+    have "fst tw < next_time_world tw"
+      by (simp add: next_time_world_at_least)
+    have "i < fst tw \<or> fst tw \<le> i"
+      by auto
+    moreover
+    { assume "i < fst tw"
+      hence "property (i + 1) i tw"
+        using \<open>inv tw\<close> unfolding inv_def by auto
+      hence "property (i + 1) i (next_world tw)"
+        unfolding property_def by simp }
+    moreover
+    { assume "fst tw \<le> i"
+      moreover have "\<forall>i \<ge> fst tw. property (i + 1) (fst tw) tw"
+        using \<open>inv2 tw\<close> \<open>disjnt {A, B} (event_of tw)\<close> unfolding inv2_def
+        by auto
+      ultimately have "property (i + 1) (fst tw) tw"
+        by auto
+      hence "property (i + 1) i tw"
+        unfolding property_def
+        by (metis \<open>get_time tw \<le> i\<close> \<open>i < next_time_world tw\<close> unchanged_until_next_time_world)
+      hence "property (i + 1) i (next_world tw)"
+        unfolding property_def by auto }
+    ultimately have "property (i + 1) i (next_world tw)"
+      by auto }
+  thus "inv (next_world tw)"
+    unfolding inv_def by auto
+qed
+
+lemma add_conc_hoare2:
+  "\<And>tw. inv tw \<and> inv2 tw \<and> disjnt {A, B} (event_of tw) \<Longrightarrow> inv2 (next_world tw)"
+proof -
+  fix tw
+  assume "inv tw \<and> inv2 tw \<and> disjnt {A, B} (event_of tw)"
+  hence "inv tw" and "inv2 tw" and "disjnt {A, B} (event_of tw)"
+    by auto
+  let ?t' = "next_time_world tw"
+  { assume "disjnt {A, B} (event_of (next_world tw))"
+    hence *: "lof_wline tw A ?t' = lof_wline tw A (?t' - 1)" and **: "lof_wline tw B ?t' = lof_wline tw B (?t' - 1)"
+      unfolding event_of_alt_def
+      by (smt comp_apply diff_0_eq_0 disjnt_insert1 fst_conv mem_Collect_eq snd_conv)+
+    have "fst tw < ?t'"
+      by (simp add: next_time_world_at_least)
+    { fix i
+      assume "?t' \<le> i"
+      have "property (i + 1) (fst tw) tw"
+        using \<open>inv2 tw\<close> \<open>disjnt {A, B} (event_of tw)\<close> unfolding inv2_def
+        using \<open>get_time tw < next_time_world tw\<close> \<open>next_time_world tw \<le> i\<close> by auto
+      moreover have "lof_wline tw A (fst tw) = lof_wline tw A (?t' - 1)" and
+                    "lof_wline tw B (fst tw) = lof_wline tw B (?t' - 1)"
+        by (metis \<open>get_time tw < next_time_world tw\<close> add_le_imp_le_diff diff_less discrete gr_implies_not0 not_less_iff_gr_or_eq unchanged_until_next_time_world zero_less_one)+
+      ultimately have "property (i + 1) ?t' (next_world tw)"
+        unfolding property_def using * **  by auto }
+    hence "\<forall>i\<ge>?t'. property (i + 1) ?t' (next_world tw)"
+      by auto }
+  thus "inv2 (next_world tw)"
+    unfolding inv2_def by auto
+qed
+
+lemma inv2_next_time:
+  fixes tw
+  assumes "beval_world_raw2 tw (Badd (Bsig A) (Bsig B)) v" and "type_of v = Lty Sig len"
+  defines "tw' \<equiv> tw[C, 1 :=\<^sub>2 v]"
+  shows   "inv2 (next_time_world tw', snd tw')"
+  unfolding inv2_def
+proof (rule, rule, rule)
+  fix i
+  assume "disjnt {A, B} (event_of (next_world tw'))"
+  hence "A \<notin> event_of (next_world tw')" and "B \<notin> event_of (next_world tw')"
+    by auto
+  assume "fst (next_world tw') \<le> i"
+  hence "next_time_world tw' \<le> i"
+    by auto
+  let ?t' = "next_time_world tw'"
+  have "fst tw' < ?t'"
+    using next_time_world_at_least by blast
+  moreover have "fst tw = fst tw'"
+    unfolding tw'_def unfolding worldline_upd2_def by auto
+  ultimately have "fst tw < ?t'"
+    by auto
+  have 0: "wline_of (next_world tw') A ?t' = wline_of tw A (fst tw)"
+  proof -
+    have "wline_of tw' A ?t' = wline_of tw' A (?t' - 1)"
+      using \<open>A \<notin> event_of (next_world tw')\<close> unfolding event_of_alt_def
+      using \<open>get_time tw' < next_time_world tw'\<close> by auto
+    also have " ... = wline_of tw' A (fst tw')"
+      using unchanged_until_next_time_world
+      by (metis (no_types, lifting) Suc_diff_1 \<open>get_time tw' < next_time_world tw'\<close> diff_less
+      gr_implies_not_zero le_0_eq less_Suc_eq_le not_less zero_less_one)
+    also have "... = wline_of tw' A (fst tw)"
+      by (simp add: \<open>get_time tw = get_time tw'\<close>)
+    also have "... = wline_of tw A (fst tw)"
+      unfolding tw'_def worldline_upd2_def worldline_upd_def by auto
+    finally show "wline_of (next_world tw') A ?t' = wline_of tw A (fst tw)"
+      by auto
+  qed
+  have 1: "wline_of (next_world tw') B ?t' = wline_of tw B (fst tw)"
+  proof -
+    have "wline_of tw' B ?t' = wline_of tw' B (?t' - 1)"
+      using \<open>B \<notin> event_of (next_world tw')\<close> unfolding event_of_alt_def
+      using \<open>get_time tw' < next_time_world tw'\<close> by auto
+    also have " ... = wline_of tw' B (fst tw')"
+      using unchanged_until_next_time_world
+      by (metis (no_types, lifting) Suc_diff_1 \<open>get_time tw' < next_time_world tw'\<close> diff_less
+      gr_implies_not_zero le_0_eq less_Suc_eq_le not_less zero_less_one)
+    also have "... = wline_of tw' B (fst tw)"
+      by (simp add: \<open>get_time tw = get_time tw'\<close>)
+    also have "... = wline_of tw B (fst tw)"
+      unfolding tw'_def worldline_upd2_def worldline_upd_def by auto
+    finally show "wline_of (next_world tw') B ?t' = wline_of tw B (fst tw)"
+      by auto
+  qed
+  have assm2: "beval_world_raw (snd tw) (fst tw) (Badd (Bsig A) (Bsig B)) v"
+    using assms(1) unfolding beval_world_raw2_def by auto
+  have "wline_of (next_world tw') C (i + 1) = v"
+  proof -
+    have "wline_of tw' C (i + 1) = v"
+      using `fst tw < ?t'` \<open>?t' \<le> i\<close>
+      unfolding tw'_def worldline_upd2_def worldline_upd_def by auto
+    thus ?thesis
+      by auto
+  qed
+  also have "lval_of ... = bin_to_bl len (sbl_to_bin (lof_wline tw A (fst tw)) + sbl_to_bin (lof_wline tw B (fst tw)))"
+    apply (rule beval_world_raw_cases[OF assm2])
+    apply (erule beval_cases)
+    defer
+    apply (metis (mono_tags, lifting) add.right_neutral assms(2) beval_cases(1) bin_to_bl_def comp_apply list.size(3) size_bin_to_bl_aux state_of_world_def ty.distinct(1) ty.inject type_of.elims val.sel(3))
+    using assms(2) by auto
+  finally have "property (i + 1) ?t' (next_world tw')"
+    unfolding property_def using 0 1  by auto
+  thus "property (i + 1) (get_time (next_time_world tw', snd tw')) (next_time_world tw', snd tw')"
+    by auto
+qed
+
+lemma add_seq_hoare_next_time1:
+  shows "\<turnstile> [\<lambda>tw. wityping \<Gamma> (snd tw)] Bassign_trans C (Badd (Bsig A) (Bsig B)) 1 [\<lambda>tw. inv2 (next_time_world tw, snd tw)]"
+  apply (rule Assign2_altI)
+  using inv2_next_time type_correctness_length by blast
+
+lemma add_conc_hoare3:
+  "\<turnstile> \<lbrace>\<lambda>tw. (inv tw \<and> wityping \<Gamma> (snd tw)) \<and> inv2 tw\<rbrace> add \<lbrace>\<lambda>tw. inv (next_time_world tw, snd tw) \<and> inv2 (next_time_world tw, snd tw)\<rbrace>"
+  unfolding add_def
+  apply (rule Single)
+   apply (rule Conj)
+    apply (rule strengthen_precondition)
+  apply (rule strengthen_precondition)
+    apply (rule add_seq_hoare_next_time)
+  apply (rule strengthen_precondition)
+   apply (rule strengthen_precondition)
+   apply (rule strengthen_precondition2)
+   apply (rule add_seq_hoare_next_time1)
+  using add_conc_hoare add_conc_hoare2 by blast
+
+lemma seq_wt_add:
+  "seq_wt \<Gamma> (Bassign_trans C (Badd (Bsig A) (Bsig B)) 1)"
+  using well_typed by blast
+
+lemma add_conc_hoare4:
+  "\<turnstile> \<lbrace>\<lambda>tw. (inv tw \<and> wityping \<Gamma> (snd tw)) \<and> inv2 tw\<rbrace> add \<lbrace>\<lambda>tw. (inv (next_time_world tw, snd tw) \<and> wityping \<Gamma> (snd tw)) \<and> inv2 (next_time_world tw, snd tw)\<rbrace>"
+  apply (rule Conj2)
+   apply (rule Conj2)
+    apply (rule weaken_post_conc_hoare[OF _ add_conc_hoare3], blast)
+   apply (rule strengthen_pre_conc_hoare[rotated])
+    apply (unfold add_def, rule single_conc_stmt_preserve_wityping_hoare)
+    apply (rule seq_wt_add)
+   apply blast
+  apply (fold add_def, rule weaken_post_conc_hoare[OF _ add_conc_hoare3], blast)
+  done
+
+lemma add_conc_sim':
+  "\<turnstile>\<^sub>s \<lbrace>\<lambda>tw. (inv tw \<and> wityping \<Gamma> (snd tw)) \<and> inv2 tw\<rbrace> add \<lbrace>\<lambda>tw. (inv tw \<and> wityping \<Gamma> (snd tw)) \<and> inv2 tw\<rbrace>"
+  apply (rule While)
+  apply (unfold snd_conv, rule add_conc_hoare4)
+  done
+
+lemma add_conc_sim2:
+  "\<turnstile>\<^sub>s \<lbrace>\<lambda>tw. (inv tw \<and> wityping \<Gamma> (snd tw)) \<and> inv2 tw\<rbrace> add \<lbrace>inv\<rbrace>"
+  using add_conc_sim' Conseq_sim by blast
+
+lemma init_sat_add_inv:
+  "init_sim_hoare (\<lambda>tw. fst tw = 0 \<and> wityping \<Gamma> (snd tw)) add (\<lambda>tw. inv tw \<and> wityping \<Gamma> (snd tw))"
+  unfolding add_def
+  apply (rule AssignI)
+  apply (rule SingleI)
+  apply (rule Conj)
+  unfolding snd_conv apply(rule add_seq_hoare_next_time0)
+  apply (rule strengthen_precondition2)
+  by (metis seq_stmt_preserve_wityping_hoare well_typed)
+
+lemma init_sat_add_inv2:
+  "init_sim_hoare (\<lambda>tw. wityping \<Gamma> (snd tw)) add inv2"
+  unfolding add_def
+  apply (rule AssignI)
+  apply (rule SingleI)
+  unfolding snd_conv apply (rule add_seq_hoare_next_time1)
+  done
+
+lemma init_sat_add_inv_comb:
+  shows "init_sim_hoare (\<lambda>tw. fst tw = 0 \<and> wityping \<Gamma> (snd tw)) add  (\<lambda>tw. (inv tw \<and> wityping \<Gamma> (snd tw)) \<and> inv2 tw)"
+  apply (rule ConjI_sim)
+  apply (rule init_sat_add_inv)
+  apply (rule ConseqI_sim[rotated])
+  apply (rule init_sat_add_inv2)
+  by blast+
+
+lemma add_correctness:
+  assumes "sim_fin w (i + 1) add tw'" and "wityping \<Gamma> w"
+  shows   "property (i + 1) i tw'"
+proof -
+  obtain tw where "init_sim (0, w) add tw" and  "tw, i + 1, add \<Rightarrow>\<^sub>S tw'"
+    using premises_sim_fin_obt[OF assms(1)] by auto
+  hence "i + 1 < fst tw'"
+    using world_maxtime_lt_fst_tres  by blast
+  have "conc_stmt_wf add"
+    unfolding conc_stmt_wf_def add_def by auto
+  moreover have "nonneg_delay_conc add"
+    unfolding add_def by auto
+  ultimately have "init_sim_valid (\<lambda>tw. fst tw = 0 \<and> wityping \<Gamma> (snd tw)) add (\<lambda>tw. (inv tw \<and> wityping \<Gamma> (snd tw)) \<and> inv2 tw)"
+    using init_sim_hoare_soundness[OF init_sat_add_inv_comb]
+    by (metis (no_types, lifting) conc_wt_cases(1) init_sat_add_inv_comb
+    init_sim_hoare_soundness add_def strengthen_precondition_init_sim_hoare)
+  hence "inv tw \<and> wityping \<Gamma> (snd tw) \<and> inv2 tw"
+    using \<open>init_sim (0, w) add tw\<close> fst_conv assms(2) unfolding init_sim_valid_def
+    by (metis snd_conv)
+  hence "inv tw" and "inv2 tw" and "wityping \<Gamma> (snd tw)"
+    by auto
+  moreover have "\<Turnstile>\<^sub>s \<lbrace>\<lambda>tw. (inv tw \<and> wityping \<Gamma> (snd tw)) \<and> inv2 tw\<rbrace> add \<lbrace>inv\<rbrace>"
+    using conc_sim_soundness[OF add_conc_sim2] \<open>conc_stmt_wf add\<close> \<open>nonneg_delay_conc add\<close>
+    by auto
+  ultimately have "inv tw'"
+    using \<open>tw, i + 1, add \<Rightarrow>\<^sub>S tw'\<close> unfolding sim_hoare_valid_def by blast
+  with \<open>i + 1 < fst tw'\<close> show ?thesis
+    unfolding inv_def by auto
+qed
+
+lemma add_correctness2:
+  assumes "sim_fin w (i + 1) add tw'" and "wityping \<Gamma> w"
+  shows   "wityping \<Gamma> (snd tw')"
+proof -
+  obtain tw where "init_sim (0, w) add tw" and  "tw, i + 1, add \<Rightarrow>\<^sub>S tw'"
+    using premises_sim_fin_obt[OF assms(1)] by auto
+  hence "i + 1 < fst tw'"
+    using world_maxtime_lt_fst_tres  by blast
+  have "conc_stmt_wf add"
+    unfolding conc_stmt_wf_def add_def by auto
+  moreover have "nonneg_delay_conc add"
+    unfolding add_def by auto
+  ultimately have "init_sim_valid (\<lambda>tw. fst tw = 0 \<and> wityping \<Gamma> (snd tw)) add (\<lambda>tw. (inv tw \<and> wityping \<Gamma> (snd tw)) \<and> inv2 tw)"
+    using init_sim_hoare_soundness[OF init_sat_add_inv_comb]
+    by (metis (no_types, lifting) conc_wt_cases(1) init_sat_add_inv_comb
+    init_sim_hoare_soundness add_def strengthen_precondition_init_sim_hoare)
+  hence "inv tw \<and> wityping \<Gamma> (snd tw) \<and> inv2 tw"
+    using \<open>init_sim (0, w) add tw\<close> fst_conv assms(2) unfolding init_sim_valid_def
+    by (metis snd_conv)
+  hence "inv tw" and "inv2 tw" and "wityping \<Gamma> (snd tw)"
+    by auto
+  moreover have "\<Turnstile>\<^sub>s \<lbrace>\<lambda>tw. (inv tw \<and> wityping \<Gamma> (snd tw)) \<and> inv2 tw\<rbrace> add \<lbrace>\<lambda>tw. wityping \<Gamma> (snd tw)\<rbrace>"
+    using conc_sim_soundness[OF add_conc_sim'] \<open>conc_stmt_wf add\<close> \<open>nonneg_delay_conc add\<close>
+    by (metis (no_types, lifting) sim_hoare_valid_def)
+  ultimately show "wityping \<Gamma> (snd tw')"
+    using \<open>tw, i + 1, add \<Rightarrow>\<^sub>S tw'\<close> unfolding sim_hoare_valid_def by blast
+qed
+
+corollary add_correctness3:
+  assumes "sim_fin w (i + 1) add tw'" and "wityping \<Gamma> w"
+  defines "bsA \<equiv> lof_wline tw' A i"
+  defines "bsB \<equiv> lof_wline tw' B i"
+  defines "bsC \<equiv> lof_wline tw' C (i + 1)"
+  assumes "2 \<le> len1" and "2 \<le> len2" \<comment> \<open>bit length of less than two is senseless for signed number\<close>
+  assumes "\<bar>sbl_to_bin bsA + sbl_to_bin bsB\<bar> < 2 ^ (len - 1)" \<comment> \<open>no overflows\<close>
+  shows   "sbl_to_bin bsC = sbl_to_bin bsA + sbl_to_bin bsB" and
+          "length bsC = len" and "2 \<le> length bsB" and  "length bsA = len1"
+proof -
+  have "property (i + 1) i tw'" and "wityping \<Gamma> (snd tw')"
+    using add_correctness[OF assms(1-2)] add_correctness2[OF assms(1-2)] by auto
+  hence "length bsA = len1" and "length bsB = len2"
+    by (smt assms(3-4) atype btype o_apply ty.distinct(1) ty.inject type_of.elims val.sel(3)
+    wityping_def wtyping_def)+
+  hence "2 \<le> length bsA" and "2 \<le> length bsB"
+    using assms by blast+
+  hence "2 \<le> len"
+    using assms unfolding len_def by auto
+  have "lof_wline tw' C (i + 1) =
+                  bin_to_bl len (sbl_to_bin (lof_wline tw' A i) + sbl_to_bin (lof_wline tw' B i))"
+    using \<open>property (i + 1) i tw'\<close> unfolding property_def by auto
+  hence "bsC = bin_to_bl len (sbl_to_bin bsA + sbl_to_bin bsB)" (is "_ = ?rhs")
+    unfolding bsA_def bsB_def bsC_def by auto
+  hence "sbl_to_bin bsC = sbl_to_bin ?rhs"
+    by auto
+  also have "... = (sbl_to_bin bsA + sbl_to_bin bsB)"
+    using sbin_bl_bin \<open>2 \<le> len\<close> assms(8) by auto
+  finally show "sbl_to_bin bsC = sbl_to_bin bsA + sbl_to_bin bsB"
+    by auto
+  show "length bsC = len" and "2 \<le> length bsB" and "length bsA = len1"
+    using \<open>bsC = bin_to_bl len (sbl_to_bin bsA + sbl_to_bin bsB)\<close> size_bin_to_bl \<open>2 \<le> length bsB\<close>
+    \<open>length bsA = len1\<close> by blast+
+qed
+
+corollary add_correctness4:
+  assumes "sim_fin w (i + 1) add tw'" and "wityping \<Gamma> w"
+  defines "bsA \<equiv> lof_wline tw' A i"
+  defines "bsB \<equiv> lof_wline tw' B i"
+  defines "bsC \<equiv> lof_wline tw' C (i + 1)"
+  assumes "2 \<le> len1" and "2 \<le> len2" \<comment> \<open>bit length of less than two is senseless for signed number\<close>
+  assumes "\<bar>sbl_to_bin bsA + sbl_to_bin bsB\<bar> < 2 ^ (len - 1)" \<comment> \<open>no overflows\<close>
+  shows   "- (int \<circ> of_bool) (hd bsC) * 2 ^ (length bsC - 1) + (\<Sum>i = 0..<length bsC - 1. (int \<circ> of_bool) (rev (tl bsC) ! i) * 2 ^ i) =
+           - (int \<circ> of_bool) (hd bsA) * 2 ^ (length bsA - 1) + (\<Sum>i = 0..<length bsA - 1. (int \<circ> of_bool) (rev (tl bsA) ! i) * 2 ^ i) +
+          (- (int \<circ> of_bool) (hd bsB) * 2 ^ (length bsB - 1) + (\<Sum>i = 0..<length bsB - 1. (int \<circ> of_bool) (rev (tl bsB) ! i) * 2 ^ i) )"
+proof -
+  have "sbl_to_bin bsC = sbl_to_bin bsA + sbl_to_bin bsB" and  "length bsC = len" and "2 \<le> length bsB" and "length bsA = len1"
+    using add_correctness3 assms by auto
+  hence "0 < length bsC"
+    unfolding len_def using \<open>2 \<le> len1\<close> \<open>2 \<le> len2\<close> by auto
+  then obtain c bsC' where "bsC = c # bsC'" and "hd bsC = c" and "tl bsC = bsC'"
+    using list.exhaust_sel by auto
+  hence sC: "sbl_to_bin bsC = - (int \<circ> of_bool) (hd bsC) * 2 ^ (length bsC - 1) + (\<Sum>i = 0..<length bsC - 1. (int \<circ> of_bool) (rev (tl bsC) ! i) * 2 ^ i)"
+    using sbl_to_bin_correctness by simp
+  obtain b bsB' a bsA' where "bsA = a # bsA'" and "bsB = b # bsB'" and "hd bsA = a" and "tl bsA = bsA'"
+    and "hd bsB = b" and "tl bsB = bsB'"
+    by (metis \<open>2 \<le> length bsB\<close> \<open>length bsA = len1\<close> assms(6) le_0_eq length_greater_0_conv
+    list.sel(1) list.sel(3) list.size(3) list_exhaust_size_gt0 zero_neq_numeral)
+  hence sA: "sbl_to_bin bsA = - (int \<circ> of_bool) (hd bsA) * 2 ^ (length bsA - 1) + (\<Sum>i = 0..<length bsA - 1. (int \<circ> of_bool) (rev (tl bsA) ! i) * 2 ^ i)"
+    and sB: "sbl_to_bin bsB = - (int \<circ> of_bool) (hd bsB) * 2 ^ (length bsB - 1) + (\<Sum>i = 0..<length bsB - 1. (int \<circ> of_bool) (rev (tl bsB) ! i) * 2 ^ i)"
+    using sbl_to_bin_correctness by simp+
+  show ?thesis
+    using \<open>sbl_to_bin bsC = sbl_to_bin bsA + sbl_to_bin bsB\<close> unfolding sA sB sC by auto
+qed
+
+end
