Bits_Int_Aux.thy
@@ -1,0 +1,190 @@
+(*
+ * Copyright 2019, NTU
+ *
+ * This software may be distributed and modified according to the terms of
+ * the BSD 2-Clause license. Note that NO WARRANTY is provided.
+ * See "LICENSE_BSD2.txt" for details.
+ *
+ *  Author: Albert Rizaldi, NTU Singapore
+ *)
+
+theory Bits_Int_Aux
+  imports
+    Main "HOL-Word.Word"
+begin
+
+text \<open>The function @{term "bl_to_bin_aux"} is the auxiliary function for converting a bit vector
+(list of booleans) into an integer with unsigned number interpretation. This semantics or conversion
+is taken from @{cite "Bryant2010"} (Chapter 2.2). Given a list x = [x_{n-1}, x_{n-2}, ... , x_0] of
+booleans with conversion False \<mapsto> 0 and True \<mapsto> 1, the unsigned number it represents is
+
+    B2U (x) \<equiv> \<Sum>i=0..<n. x_i * 2 ^ i   .
+
+The following lemma formalises this correctness.\<close>
+
+lemma bl_to_bin_aux_correctness:
+  " bl_to_bin_aux bs w =  w * 2 ^ length bs + (\<Sum>i = 0..<length bs. (int \<circ> of_bool) (rev bs ! i) * 2 ^ i)"
+proof (induction bs arbitrary: w)
+  case Nil
+  then show ?case by auto
+next
+  case (Cons a bs)
+    \<comment> \<open>from left hand side\<close>
+  have " bl_to_bin_aux (a # bs) w = bl_to_bin_aux bs (w BIT a)"
+    by auto
+  also have "... =  (w BIT a) * 2 ^ length bs + (\<Sum>i = 0..<length bs. (int \<circ> of_bool) (rev bs ! i) * 2 ^ i)" (is "_ = _ + ?rhs2")
+    using Cons by auto
+  also have "... = (2 * w + (int o of_bool) a) * 2 ^ length bs + ?rhs2"
+    unfolding Bit_def by auto
+  also have "... = w * 2 ^ (length (a # bs)) + (int o of_bool) a * 2 ^ length bs + ?rhs2"
+    by (auto simp add: field_simps)
+  also have "... = w * 2 ^ length (a # bs) + (\<Sum>i = 0..<length (a # bs). (int \<circ> of_bool) (rev (a # bs) ! i) * 2 ^ i)"
+  proof -
+    have "(\<Sum>i = 0..<length (a # bs). (int \<circ> of_bool) (rev (a # bs) ! i) * 2 ^ i) =
+          (\<Sum>i = 0..<Suc (length bs). (int \<circ> of_bool) (rev (a # bs) ! i) * 2 ^ i) "
+      by auto
+    also have "... = (\<Sum>i = 0..<length bs. (int \<circ> of_bool) (rev (a # bs) ! i) * 2 ^ i) + (int \<circ> of_bool) a * 2 ^ length bs "
+      using nth_rev_alt by fastforce
+    also have "... = (\<Sum>i= 0..< length bs. (int o of_bool) (rev bs ! i) * 2 ^ i) + (int o of_bool) a * 2 ^ length bs"
+      unfolding cancel_semigroup_add_class.add_right_cancel
+    proof (intro sum.mono_neutral_cong)
+      fix x
+      assume "x \<in> {0..<length bs} \<inter> {0..<length bs}"
+      hence "x \<in> {0 ..< length bs}"
+        by auto
+      thus "(int \<circ> of_bool) (rev (a # bs) ! x) * 2 ^ x = (int \<circ> of_bool) (rev bs ! x) * 2 ^ x"
+        by (smt atLeastLessThan_iff bin_nth_of_bl_aux bl_to_bin_aux.simps(2) length_Cons less_Suc_eq not_less)
+    qed (auto)
+    finally show ?thesis
+      by auto
+  qed
+  finally show ?case
+    by auto
+qed
+
+lemma bl_to_bin_correctness:
+  "bl_to_bin bs = (\<Sum>i = 0..<length bs. (int \<circ> of_bool) (rev bs ! i) * 2 ^ i)"
+  unfolding bl_to_bin_def using bl_to_bin_aux_correctness by auto
+
+text \<open> In case it is interpreted as unsigned number, the equation is
+
+    B2S (x) \<equiv> - x_{n-1} * 2 ^ {n - 1} + \<Sum>i=0..<n-1. x_i * 2 ^ i .
+
+Note that the most significant bit has the value of (- 2 ^ {n - 1}) instead of (2 ^ {n - 1}).
+Unfortunately there is no such function in @{theory "HOL-Word.Bits_Int"}. Fortunately we can
+easily obtain such function with simple arithmetic as follows.
+\<close>
+
+fun sbl_to_bin :: "bool list \<Rightarrow> int" where
+  "sbl_to_bin [] = 0"
+| "sbl_to_bin bs = bl_to_bin bs - (int o of_bool) (hd bs) * 2 ^ (length bs)"
+
+text \<open>This is the correctness theorem according to the definition of B2S. \<close>
+
+lemma sbl_to_bin_correctness:
+  "sbl_to_bin (a # bs) = - (int o of_bool) a * 2 ^ (length bs) + (\<Sum>i = 0 ..< length bs. ((int o of_bool) (rev bs ! i)) * 2 ^ i) "
+proof -
+  have "sbl_to_bin (a # bs) = bl_to_bin (a # bs) - (int o of_bool) a * 2 ^ (1 + length bs)"
+    by auto
+  also have "... = bl_to_bin (a # bs) - 2 * (int o of_bool) a * 2 ^ length bs"
+    by auto
+  also have "... = (\<Sum>i = 0..< Suc (length bs). (int \<circ> of_bool) (rev (a # bs) ! i) * 2 ^ i) - 2 * (int o of_bool) a * 2 ^ length bs"
+    unfolding bl_to_bin_correctness by auto
+  also have "... = (\<Sum>i = 0..< length bs. (int \<circ> of_bool) (rev (a # bs) ! i) * 2 ^ i) + (int o of_bool) a * 2 ^ length bs - 2 * (int o of_bool) a * 2 ^ length bs"
+    using list.size(4) nth_rev_alt by fastforce
+  also have "... = (\<Sum>i = 0..< length bs. (int \<circ> of_bool) (rev (a # bs) ! i) * 2 ^ i) - (int o of_bool) a * 2 ^ length bs"
+    by auto
+  also have "... = (\<Sum>i = 0..< length bs. (int \<circ> of_bool) (rev bs ! i) * 2 ^ i) - (int o of_bool) a * 2 ^ length bs"
+  proof -
+    have "(\<Sum>i = 0..<length bs. (int \<circ> of_bool) (rev (a # bs) ! i) * 2 ^ i) =
+          (\<Sum>i = 0..<length bs. (int \<circ> of_bool) (rev bs ! i) * 2 ^ i)"
+      apply (intro sum.mono_neutral_cong[rotated 4])
+      by (smt One_nat_def add.commute atLeastLessThan_iff bin_nth_of_bl bin_nth_of_bl_aux
+      bl_to_bin_aux.Cons inf.idem less_Suc_eq list.size(4) not_less plus_1_eq_Suc) auto
+    thus ?thesis
+      by auto
+  qed
+  finally show ?thesis
+    by auto
+qed
+
+lemma sign_bit_is_0:
+  assumes "0 \<le> w" and "w < 2 ^ len"
+  shows   "hd (bin_to_bl (Suc len) w) = False"
+  using assms sbintrunc_mod2p sign_Min_lt_0 unfolding bl_sbin_sign by auto
+
+lemma sign_bit_is_1:
+  assumes "w < 0" and "- w < 2 ^ len"
+  shows   "hd (bin_to_bl (Suc len) w) = True"
+  using assms bin_sign_def no_sbintr_alt2 unfolding bl_sbin_sign by auto
+
+lemma sbin_bl_bin:
+  assumes "0 < n" and "\<bar>w\<bar> < 2 ^ (n - 1)"
+  shows "sbl_to_bin (bin_to_bl n w) = w"
+proof -
+  obtain a bs where "bin_to_bl n w = (a # bs)"
+    using assms  size_bin_to_bl  by (metis list.size(3) not_less_zero sbl_to_bin.cases)
+  have "sbl_to_bin (bin_to_bl n w) = sbl_to_bin (a # bs)"
+    using \<open>bin_to_bl n w = (a # bs)\<close> by auto
+  also have "... = - (int o of_bool) a * 2 ^ (length bs)
+                 + (\<Sum>i = 0 ..< length bs. ((int o of_bool) (rev bs ! i)) * 2 ^ i)"
+    unfolding sbl_to_bin_correctness by auto
+  finally have "sbl_to_bin (bin_to_bl n w) = - (int o of_bool) a * 2 ^ (length bs)
+                                           + (\<Sum>i = 0 ..< length bs. ((int o of_bool) (rev bs ! i)) * 2 ^ i)"
+    by auto
+  have "sbl_to_bin (bin_to_bl n w) = sbl_to_bin (a # bs)"
+    using \<open>bin_to_bl n w = a # bs\<close> by auto
+  also have "... = bl_to_bin (a # bs) - (int o of_bool) a * 2 ^ (1 + length bs)"
+    by auto
+  also have "... = bl_to_bin (bin_to_bl n w) - (int o of_bool) a * 2 ^ (1 + length bs)"
+    using \<open>bin_to_bl n w = a # bs\<close> by auto
+  also have "... = bintrunc n w - (int o of_bool) a * 2 ^ (1 + length bs)"
+    unfolding bin_bl_bin by auto
+  also have "... = w mod (2 ^ n) - (int o of_bool) a * 2 ^ (1 + length bs)"
+    by (simp add: no_bintr_alt1)
+  also have "... = w mod (2 ^ n) - (int o of_bool) a * 2 ^ n"
+    by (metis \<open>bin_to_bl n w = a # bs\<close> length_Cons plus_1_eq_Suc size_bin_to_bl)
+  also have "... = w"
+  proof (cases "0 \<le> w")
+    case True
+    hence "a = False"
+      using sign_bit_is_0
+      by (smt One_nat_def \<open>bin_to_bl n w = a # bs\<close> add.commute add_diff_cancel_left' assms(2)
+      length_Cons list.sel(1) list.size(4) size_bin_to_bl)
+    then show ?thesis
+      by (smt Bit_B1_2t One_nat_def True \<open>bin_to_bl n w = a # bs\<close> add.commute add_diff_cancel_left'
+      assms(2) comp_apply int_mod_eq' list.size(4) mult_eq_0_iff of_bool_eq(1) plus_1_eq_Suc
+      power_BIT semiring_1_class.of_nat_0 size_bin_to_bl)
+  next
+    case False
+    hence "a = True"
+      using sign_bit_is_1
+      by (smt One_nat_def \<open>bin_to_bl n w = a # bs\<close> add.commute add_diff_cancel_left' assms(2)
+      list.sel(1) list.size(4) plus_1_eq_Suc size_bin_to_bl)
+    obtain w' where "w = -w'"
+      using False  by (metis add.inverse_inverse)
+    hence *: "- w' mod 2 ^ n = (if w' mod 2 ^ n = 0 then 0 else 2 ^ n - w' mod 2 ^ n)"
+      unfolding zmod_zminus1_eq_if by auto
+    have "w' < 2 ^ n"
+      by (smt One_nat_def \<open>bin_to_bl n w = a # bs\<close> \<open>w = - w'\<close> add.commute add_diff_cancel_left'
+      assms(2) less_Suc_eq list.size(4) plus_1_eq_Suc power_strict_increasing_iff size_bin_to_bl)
+    hence "w' mod 2 ^ n \<noteq> 0"
+      using False \<open>w = - w'\<close> by auto
+    hence "- w' mod 2 ^ n = 2 ^ n - (w' mod 2 ^ n)"
+      using * by auto
+    hence "w mod 2 ^ n = 2 ^ n - (\<bar>w\<bar> mod 2 ^ n)"
+      using False \<open>w = - w'\<close> by auto
+    hence "w mod 2 ^ n - (int \<circ> of_bool) a * 2 ^ n = 2 ^ n - (\<bar>w\<bar> mod 2 ^ n) - 2 ^ n"
+      by (simp add: \<open>a = True\<close>)
+    also have "... = - (\<bar>w\<bar> mod 2 ^ n)"
+      by auto
+    also have "... = w"
+      using False \<open>w = - w'\<close> \<open>w' < 2 ^ n\<close> by auto
+    finally show ?thesis
+      by auto
+  qed
+  finally show ?thesis
+    by auto
+qed
+
+end
