Slicing_Hoare.thy
@@ -19,38 +19,38 @@ definition slicer :: "sig conc_stmt" where
 
 lemma potential_tyenv:
   assumes "seq_wt \<Gamma> (Bassign_trans OUT (Bslice IN 3 2) 1)"
-  shows "\<exists>len>3. \<Gamma> IN = Lty len \<and> \<Gamma> OUT = Lty 2"
+  shows "\<exists>ki len. 3 < len \<and> \<Gamma> IN = Lty ki len \<and> \<Gamma> OUT = Lty ki 2"
 proof (rule seq_wt_cases(4)[OF assms])
   assume "bexp_wt \<Gamma> (Bslice IN 3 2) (\<Gamma> OUT)"
-  then obtain len where "bexp_wt \<Gamma> (Bsig IN) (Lty len) \<and> 3 < len \<and> \<Gamma> OUT = Lty 2"
+  then obtain ki len where "bexp_wt \<Gamma> (Bsig IN) (Lty ki len) \<and> 3 < len \<and> \<Gamma> OUT = Lty ki 2"
     by (metis add_2_eq_Suc add_Suc add_Suc_right add_diff_cancel_right' bexp_wt_cases(8)
     numeral_2_eq_2 numeral_3_eq_3)
-  hence "bexp_wt \<Gamma> (Bsig IN) (Lty len)" and "3 < len" and "\<Gamma> OUT = Lty 2"
+  hence "bexp_wt \<Gamma> (Bsig IN) (Lty ki len)" and "3 < len" and "\<Gamma> OUT = Lty ki 2"
     by auto
-  hence "\<Gamma> IN = Lty len"
-    using bexp_wt_cases(9)[OF \<open>bexp_wt \<Gamma> (Bsig IN) (Lty len)\<close>] by metis
+  hence "\<Gamma> IN = Lty ki len"
+    using bexp_wt_cases(9)[OF \<open>bexp_wt \<Gamma> (Bsig IN) (Lty ki len)\<close>] by metis
   thus ?thesis
-    using \<open>3 < len\<close> \<open>\<Gamma> OUT = Lty 2\<close> by blast
+    using \<open>3 < len\<close> \<open>\<Gamma> OUT = Lty ki 2\<close> by blast
 qed
 
 abbreviation "lof_wline tw sig i \<equiv> lval_of (wline_of tw sig i)"
 
 definition inv :: "sig assn2" where
-  "inv tw = (\<forall>i < fst tw. let ins = lof_wline tw IN i; idx = length ins - 1 in 
+  "inv tw = (\<forall>i < fst tw. let ins = lof_wline tw IN i; idx = length ins - 1 in
                                           lof_wline tw OUT (i + 1) = nths ins {idx - 3 .. idx - 2})"
 
 definition inv' :: "sig assn2" where
-  "inv' tw = (disjnt {IN} (event_of tw) \<longrightarrow> 
-              (\<forall>i\<ge>fst tw. let ins = lof_wline tw IN (fst tw); idx = length ins - 1 in 
+  "inv' tw = (disjnt {IN} (event_of tw) \<longrightarrow>
+              (\<forall>i\<ge>fst tw. let ins = lof_wline tw IN (fst tw); idx = length ins - 1 in
                                          lof_wline tw OUT (i + 1) = nths ins {idx - 3 .. idx - 2}))"
 
-text \<open>Note that we need the assumption that @{term "type_of x = Lty 2"} as there is no
-guarantee that @{term "beval_world_raw2 tw (Bslice IN 3 2) x"} would result in a list 
+text \<open>Note that we need the assumption that @{term "type_of x = Lty ki 2"} as there is no
+guarantee that @{term "beval_world_raw2 tw (Bslice IN 3 2) x"} would result in a list
 of length 2.\<close>
 
 lemma inv_next_time:
   assumes "inv tw"
-  assumes "beval_world_raw2 tw (Bslice IN 3 2) x" and "type_of x = Lty 2"
+  assumes "beval_world_raw2 tw (Bslice IN 3 2) x" and "type_of x = Lty ki 2"
   defines "tw' \<equiv> tw[OUT, 1 :=\<^sub>2 x]"
   shows   "inv (next_time_world tw', snd tw')"
 proof -
@@ -63,7 +63,7 @@ proof -
   have "\<forall>i < next_time_world tw'. let ins = lof_wline tw' IN i; idx = length ins - 1 in
                                            lof_wline tw' OUT (i + 1) = nths ins {idx - 3 .. idx - 2}"
   proof (rule, rule)
-    fix i 
+    fix i
     let ?ins   = "lof_wline tw IN i"
     let ?ins'  = "lof_wline tw' IN i"
     let ?instw = "lof_wline tw IN (fst tw)"
@@ -96,16 +96,16 @@ proof -
       hence "lof_wline tw' OUT (i + 1) = lof_wline tw' OUT (fst tw + 1)"
         using unchanged_until_next_time_world
         by (metis (mono_tags, lifting) Suc_eq_plus1 \<open>get_time tw = get_time tw'\<close> le_Suc_eq le_add1
-        le_less_trans less_diff_conv)      
+        le_less_trans less_diff_conv)
       have "lof_wline tw' IN i = lof_wline tw IN (fst tw)"
-        using unchanged_until_next_time_world 
+        using unchanged_until_next_time_world
         by (metis \<open>get_time tw = get_time tw'\<close> \<open>get_time tw \<le> i \<and> i < next_time_world tw' - 1\<close> \<open>i <
         next_time_world tw'\<close> less_add_one tw'_def worldline_upd2_before_dly)
       let ?instw = "lof_wline tw IN (fst tw)"
       let ?idxtw = "length ?instw - 1"
       have "nths ?ins' {?idx' - 3 .. ?idx' - 2} = nths ?instw {?idxtw - 3 .. ?idxtw - 2}"
         using \<open>lof_wline tw' IN i = lof_wline tw IN (fst tw)\<close> by simp
-      have "lof_wline tw' OUT (fst tw + 1) = lval_of x"  
+      have "lof_wline tw' OUT (fst tw + 1) = lval_of x"
         using assms(4)  by (metis worldline_upd2_at_dly)
       also have "... = nths ?instw {?idxtw - 3 .. ?idxtw - 2}"
       proof -
@@ -114,11 +114,11 @@ proof -
         have "\<not> is_Bv (wline_of tw IN (fst tw))"
           apply (rule beval_world_raw_cases[OF assms2], erule beval_cases)
           by (metis beval_cases(1) comp_apply state_of_world_def val.disc(2))
-        hence "state_of_world (snd tw) (fst tw) IN = Lv ?instw"
-          unfolding state_of_world_def by simp
+        then obtain ki where "state_of_world (snd tw) (fst tw) IN = Lv ki ?instw"
+          unfolding state_of_world_def  by (metis comp_def val.collapse(2))
         show "lval_of x = nths ?instw {?idxtw - 3 .. ?idxtw - 2}"
           apply (rule beval_world_raw_cases[OF assms2], erule beval_cases)
-          using \<open>state_of_world (snd tw) (fst tw) IN = Lv ?instw\<close> plus_1_eq_Suc by auto
+          using \<open>state_of_world (snd tw) (fst tw) IN = Lv ki ?instw\<close> plus_1_eq_Suc by auto
       qed
       also have "... = nths ?ins' {?idx' - 3 .. ?idx' - 2}"
         using \<open>lof_wline tw' IN i = lof_wline tw IN (fst tw)\<close>
@@ -144,11 +144,11 @@ proof -
         have "\<not> is_Bv (wline_of tw IN (fst tw))"
           apply (rule beval_world_raw_cases[OF assms2], erule beval_cases)
           by (metis beval_cases(1) comp_apply state_of_world_def val.disc(2))
-        hence "state_of_world (snd tw) (fst tw) IN = Lv ?instw"
-          unfolding state_of_world_def by simp
+        then obtain ki where "state_of_world (snd tw) (fst tw) IN = Lv ki ?instw"
+          unfolding state_of_world_def  by (metis comp_def val.collapse(2))
         show "lval_of x = nths ?instw {?idxtw - 3 .. ?idxtw - 2}"
           apply (rule beval_world_raw_cases[OF assms2], erule beval_cases)
-          using \<open>state_of_world (snd tw) (fst tw) IN = Lv ?instw\<close> plus_1_eq_Suc by auto
+          using \<open>state_of_world (snd tw) (fst tw) IN = Lv ki ?instw\<close> plus_1_eq_Suc by auto
       qed
       also have "... = nths ?ins' {?idx' - 3 .. ?idx' - 2}"
         by (smt \<open>get_time tw = get_time tw'\<close> \<open>i < get_time tw \<Longrightarrow> lof_wline tw' OUT (i + 1) = nths
@@ -168,33 +168,33 @@ lemma type_correctness_length:
   assumes "seq_wt \<Gamma> (Bassign_trans OUT (Bslice IN 3 2) 1)"
   assumes "wityping \<Gamma> (snd tw)"
   assumes "beval_world_raw2 tw (Bslice IN 3 2) x"
-  shows   "type_of x = Lty 2"
-proof - 
-  obtain len where "\<Gamma> IN = Lty len" and "3 < len"
+  shows   "\<exists>ki. type_of x = Lty ki 2"
+proof -
+  obtain ki len where "\<Gamma> IN = Lty ki len" and "3 < len"
     using potential_tyenv[OF assms(1)] by auto
   have *: "beval_world_raw (snd tw) (fst tw) (Bslice IN 3 2) x"
     using assms(3) unfolding beval_world_raw2_def by auto
-  have "type_of (state_of_world (snd tw) (get_time tw) IN) = Lty len"
-    using assms(2) unfolding wityping_def 
-    by (simp add: \<open>\<Gamma> IN = Lty len\<close> state_of_world_def wtyping_def)
-  hence **: "\<And>bs. state_of_world (snd tw) (fst tw) IN = Lv bs \<Longrightarrow> length bs = len"
+  have "type_of (state_of_world (snd tw) (get_time tw) IN) = Lty ki len"
+    using assms(2) unfolding wityping_def
+    by (simp add: \<open>\<Gamma> IN = Lty ki len\<close> state_of_world_def wtyping_def)
+  hence **: "\<And>bs. state_of_world (snd tw) (fst tw) IN = Lv ki bs \<Longrightarrow> length bs = len"
     by simp
   have ***: "\<And>bs. 3 < length bs  \<Longrightarrow> length (nths bs {length bs - Suc 3..length bs - Suc 2}) = 2"
   proof -
     fix bs :: "'a list"
     assume "3 < length bs"
-    hence "length (nths bs {length bs - Suc 3..length bs - Suc 2}) = 
+    hence "length (nths bs {length bs - Suc 3..length bs - Suc 2}) =
                                card {i. i < length bs \<and> i \<in> {length bs - Suc 3..length bs - Suc 2}}"
       unfolding length_nths by auto
     have "\<And>i. i \<in> {length bs - Suc 3 .. length bs - Suc 2} \<Longrightarrow> i < length bs"
       using \<open>3 < length bs\<close> by auto
-    hence "{i. i < length bs \<and> i \<in> {length bs - Suc 3 .. length bs - Suc 2}} = 
+    hence "{i. i < length bs \<and> i \<in> {length bs - Suc 3 .. length bs - Suc 2}} =
            {i. i \<in> {length bs - Suc 3 .. length bs - Suc 2}}" (is "?lhs = ?rhs")
       by auto
     hence "card ?lhs = card ?rhs"
       by auto
     also have "... = 2"
-      using \<open>3 < length bs\<close> 
+      using \<open>3 < length bs\<close>
       by (metis Collect_mem_eq One_nat_def Suc_diff_Suc Suc_numeral add_diff_cancel_left'
       add_diff_cancel_right' card_atLeastAtMost diff_less_Suc numeral_2_eq_2 plus_1_eq_Suc
       semiring_norm(5))
@@ -207,7 +207,9 @@ proof -
   show ?thesis
     apply (rule beval_world_raw_cases[OF *])
     apply (erule beval_cases)+
-    using \<open>3 < len\<close> ** ***  by force
+    using \<open>3 < len\<close> ** ***
+    by (metis \<open>type_of (state_of_world (snd tw) (get_time tw) IN) = Lty ki len\<close> ty.inject
+    type_of.simps(2))
 qed
 
 lemma slicer_seq_hoare_next_time:
@@ -220,7 +222,7 @@ lemma slicer_seq_hoare_next_time0:
   assumes "seq_wt \<Gamma> (Bassign_trans OUT (Bslice IN 3 2) 1)"
   shows "\<turnstile> [\<lambda>tw. fst tw = 0 \<and> wityping \<Gamma> (snd tw)] Bassign_trans OUT (Bslice IN 3 2) 1 [\<lambda>tw. inv (next_time_world tw, snd tw)]"
   apply (rule Assign2_altI)
-  using inv_next_time type_correctness_length[OF assms] inv_def gr_implies_not0 by blast
+  using inv_next_time type_correctness_length[OF assms] inv_def gr_implies_not0 by metis
 
 lemma slicer_conc_hoare:
   "\<And>tw. inv tw \<and> inv' tw \<and> disjnt {IN} (event_of tw) \<Longrightarrow> inv (next_time_world tw, snd tw)"
@@ -229,14 +231,14 @@ lemma slicer_conc_hoare:
 
 lemma slicer_conc_hoare2:
   "\<And>tw. inv tw \<and> inv' tw \<and> disjnt {IN} (event_of tw) \<Longrightarrow> inv' (next_time_world tw, snd tw)"
-  unfolding inv_def inv'_def 
+  unfolding inv_def inv'_def
   by (smt Suc_diff_1 comp_apply diff_less disjnt_insert1 event_of_alt_def gr_implies_not_zero
   le_Suc_eq le_less_trans mem_Collect_eq next_time_world_at_least not_less order.strict_iff_order
   prod.sel(1) snd_conv unchanged_until_next_time_world zero_less_one)
 
 lemma inv'_next_time:
   fixes tw
-  assumes "beval_world_raw2 tw (Bslice IN 3 2) x" and "type_of x = Lty 2"
+  assumes "beval_world_raw2 tw (Bslice IN 3 2) x" and "type_of x = Lty ki 2"
   defines "tw' \<equiv> tw[OUT, 1 :=\<^sub>2 x]"
   shows   "inv' (next_time_world tw', snd tw')"
   unfolding inv'_def
@@ -264,7 +266,7 @@ proof (rule, rule, rule)
       using \<open>IN \<notin> event_of (?t', snd tw')\<close> unfolding event_of_alt_def
       using \<open>get_time tw < next_time_world tw'\<close> by auto
     also have "... = wline_of tw' IN (fst tw')"
-      using unchanged_until_next_time_world 
+      using unchanged_until_next_time_world
       by (metis (no_types, lifting) Suc_diff_1 \<open>get_time tw' < next_time_world tw'\<close> diff_less
       gr_implies_not_zero le_0_eq less_Suc_eq_le not_less zero_less_one)
     also have "... = wline_of tw' IN (fst tw)"
@@ -290,14 +292,14 @@ proof (rule, rule, rule)
     have "\<not> is_Bv (wline_of tw IN (fst tw))"
       by (rule beval_world_raw_cases[OF assms2], erule beval_cases)
          (metis beval_cases(1) comp_apply state_of_world_def val.disc(2))
-    hence "state_of_world (snd tw) (fst tw) IN = Lv ?ins"
-      unfolding \<open>?ins = lof_wline tw IN (fst tw)\<close>state_of_world_def by simp
+    then obtain ki where "state_of_world (snd tw) (fst tw) IN = Lv ki ?ins"
+      unfolding \<open>?ins = lof_wline tw IN (fst tw)\<close>state_of_world_def
+      by (metis comp_def val.collapse(2))
     have "lval_of x = nths ?ins {?idx - 3 .. ?idx - 2}"
-      apply (rule beval_world_raw_cases[OF assms2])  
+      apply (rule beval_world_raw_cases[OF assms2])
       apply (erule beval_cases)+
-      using \<open>state_of_world (snd tw) (fst tw) IN = Lv ?ins\<close> 
-      by (metis \<open>lof_wline (next_time_world tw', snd tw') IN (next_time_world tw') = lof_wline tw IN
-      (get_time tw)\<close> diff_Suc_eq_diff_pred eval_nat_numeral(3) val.sel(2))
+      using \<open>state_of_world (snd tw) (fst tw) IN = Lv ki ?ins\<close>
+      by (metis diff_Suc_eq_diff_pred val.sel(3))
     thus "lof_wline tw' OUT (i + 1) = nths ?ins {?idx - 3 .. ?idx - 2}"
       using \<open>lof_wline tw' OUT (i + 1) = lval_of x\<close> by auto
   qed
@@ -318,7 +320,7 @@ lemma slicer_conc_hoare3:
   unfolding slicer_def
   apply (rule Single)
    apply (rule Conj)
-  apply (rule strengthen_precondition)    
+  apply (rule strengthen_precondition)
     apply (rule strengthen_precondition)
     apply (rule slicer_seq_hoare_next_time[OF assms])
    apply (rule strengthen_precondition)
@@ -338,7 +340,7 @@ lemma slicer_conc_hoare4:
     apply (unfold slicer_def, rule single_conc_stmt_preserve_wityping_hoare[OF assms], blast)
   apply (fold slicer_def, rule weaken_post_conc_hoare[OF _ slicer_conc_hoare3[OF assms]], blast)
   done
-  
+
 lemma slicer_conc_sim':
   assumes "seq_wt \<Gamma> (Bassign_trans OUT (Bslice IN 3 2) 1)"
   shows   "\<turnstile>\<^sub>s \<lbrace>\<lambda>tw. (inv tw \<and> wityping \<Gamma> (snd tw)) \<and> inv' tw\<rbrace> slicer \<lbrace>\<lambda>tw. (inv tw \<and> wityping \<Gamma> (snd tw)) \<and> inv' tw\<rbrace>"
@@ -383,7 +385,7 @@ lemma init_sat_slicer_inv_comb:
 lemma slicer_correctness:
   assumes "sim_fin w (i + 1) slicer tw'" and "wityping \<Gamma> w"
   assumes "conc_wt \<Gamma> slicer"
-  shows   "let ins = lof_wline tw' IN i; idx = length ins - 1 in 
+  shows   "let ins = lof_wline tw' IN i; idx = length ins - 1 in
                                           lof_wline tw' OUT (i + 1) = nths ins {idx - 3 .. idx - 2}"
 proof -
   obtain tw where "init_sim (0, w) slicer tw" and  "tw, i + 1, slicer \<Rightarrow>\<^sub>S tw'"
@@ -395,7 +397,7 @@ proof -
   moreover have "nonneg_delay_conc slicer"
     unfolding slicer_def by auto
   ultimately have "init_sim_valid (\<lambda>tw. fst tw = 0 \<and> wityping \<Gamma> (snd tw)) slicer (\<lambda>tw. (inv tw \<and> wityping \<Gamma> (snd tw)) \<and> inv' tw)"
-    using init_sim_hoare_soundness[OF init_sat_slicer_inv_comb] 
+    using init_sim_hoare_soundness[OF init_sat_slicer_inv_comb]
     by (metis (no_types, lifting) assms(3) conc_wt_cases(1) init_sat_slicer_inv_comb
     init_sim_hoare_soundness slicer_def strengthen_precondition_init_sim_hoare)
   hence "inv tw \<and> wityping \<Gamma> (snd tw) \<and> inv' tw"
@@ -413,5 +415,5 @@ proof -
   with \<open>i + 1 < fst tw'\<close> show ?thesis
     unfolding inv_def by auto
 qed
-  
+
 end
